theories/Weakening.v
@@ -1,6 +1,297 @@
-From MetaCoq.PCUIC Require Import PCUICAst.
+From MetaCoq.PCUIC Require Import PCUICAst PCUICRenameConv PCUICSigmaCalculus PCUICInstConv.
+From LogRel Require Import Notations Automation Untyped MLTTTyping.
 
-Definition isRel t :=
-    match t with tRel _ => true | _ => false end.
+Inductive weakening : Set :=
+  | wk_id : weakening
+  | wk_step (w : weakening) : weakening
+  | wk_lift (w : weakening) : weakening.
 
-Definition eta {A B : Type} (f : A -> B) : f = (fun x => f x) := eq_refl.
+(* Transforms an (intentional) weakening into a renaming *)
+Fixpoint wk_to_ren (ρ : weakening) : nat -> nat :=
+  match ρ with
+    | wk_id => id
+    | wk_step ρ' => S ∘ (wk_to_ren ρ')
+    | wk_lift ρ' => shiftn 1 (wk_to_ren ρ')
+  end.
+Coercion wk_to_ren : weakening >-> Funclass.
+
+Inductive well_weakening : weakening -> context -> context -> Type :=
+  | well_id (Γ : context) : well_weakening wk_id Γ Γ
+  | well_step (Γ Δ : context) (na : aname) (A : term) (ρ : weakening) :
+    well_weakening ρ Γ Δ -> well_weakening (wk_step ρ) (Γ,,vass na A) Δ
+  | well_lift (Γ Δ : context) (na : aname) (A : term) (ρ : weakening) :
+    well_weakening ρ Γ Δ -> well_weakening (wk_lift ρ) (Γ,,vass na (A.[ren ρ])) (Δ,, vass na A).
+
+Fixpoint wk_compose (ρ ρ' : weakening) : weakening :=
+  match ρ, ρ' with
+    | wk_id, _ => ρ'
+    | wk_step ν , _ => wk_step (wk_compose ν ρ')
+    | wk_lift ν, wk_id => ρ
+    | wk_lift ν, wk_step ν' => wk_step (wk_compose ν ν')
+    | wk_lift ν, wk_lift ν' => wk_lift (wk_compose ν ν')
+  end.
+
+Lemma wk_compose_compose (ρ ρ' : weakening) : (wk_compose ρ ρ' : nat -> nat) =1 ρ ∘ ρ'.
+Proof.
+  induction ρ in ρ' |- *.
+  - reflexivity.
+  - cbn.
+    intros ?.
+    now rewrite IHρ.
+  - destruct ρ'.
+    + reflexivity.
+    + intros n.
+      cbn.
+      now rewrite IHρ, Nat.sub_0_r.
+    + intros [] ; cbn.
+      1: reflexivity.
+      repeat rewrite Nat.sub_0_r.
+      now rewrite IHρ.
+Qed.
+
+Lemma well_wk_compose {ρ ρ' : weakening} {Δ Δ' Δ'' : context} :
+  well_weakening ρ Δ Δ' -> well_weakening ρ' Δ' Δ'' -> well_weakening (wk_compose ρ ρ') Δ Δ''.
+Proof.
+  intros H H'.
+  induction H as [| | ? ? ? ? ν] in ρ', Δ'', H' |- *.
+  all: cbn.
+  - eassumption.
+  - now econstructor.
+  - inversion H' as [| | ? ? na' A' ν'] ; subst ; clear H'.
+    1-2: now econstructor.
+    rewrite inst_assoc.
+    replace (A'.[ren ν' ∘s ren ν]) with (A'.[ren (wk_compose ν ν')]) by
+      now rewrite compose_ren, wk_compose_compose.
+    now econstructor.
+Qed.
+
+#[projections(primitive)]Record wk_well_wk {Γ Δ : context} :=
+  { wk :> weakening ; well_wk :> well_weakening wk Γ Δ}.
+Arguments wk_well_wk : clear implicits.
+Arguments Build_wk_well_wk : clear implicits.
+Notation "Γ ≤ Δ" := (wk_well_wk Γ Δ).
+
+#[global] Hint Resolve well_wk : core.
+
+Definition wk_well_wk_compose {Γ Γ' Γ'' : context} (ρ : Γ ≤ Γ') (ρ' : Γ' ≤ Γ'') : Γ ≤ Γ'' :=
+  {| wk := wk_compose ρ.(wk) ρ'.(wk) ; well_wk := well_wk_compose ρ.(well_wk) ρ'.(well_wk) |}.
+Notation "ρ ∘w ρ'" := (wk_well_wk_compose ρ ρ').
+
+
+Lemma well_length {Γ Δ : context} (ρ : Γ ≤ Δ) : #|Δ| <= #|Γ|.
+Proof.
+  destruct ρ as [ρ wellρ].
+  induction wellρ.
+  all: cbn ; lia.
+Qed.
+
+(* Testing that the definitions are right *)
+Lemma id_ren (Γ : context) (ρ : Γ ≤ Γ) : (wk_to_ren ρ) =1 id.
+Proof.
+  destruct ρ as [ρ wellρ].
+  cbn in *.
+  pose proof (@eq_refl _ #|Γ|) as eΓ.
+  revert eΓ wellρ.
+  generalize Γ at 2 4.
+  intros Δ e wellρ.
+  induction wellρ in e |- *.
+  all: cbn.
+  - reflexivity.
+  - pose proof (well_length {| wk := ρ ; well_wk := wellρ |}).
+    now cbn in * ; lia.
+  - etransitivity.
+    2: eapply shiftn_id.
+    now rewrite IHwellρ.
+Qed.
+
+Section TypingWk.
+
+Variable foo : context_decl.
+
+Lemma nth_error_wk (Γ Δ : context) n decl (ρ : Δ ≤ Γ) :
+  nth_error Γ n = Some decl ->
+  {decl' & nth_error Δ (ρ n) = Some decl' ×
+    map_decl (rename (ρ ∘ rshiftk (S n))) decl = map_decl (rename (rshiftk (S (ρ n)))) decl'}.
+Proof.
+  intros Hdecl.
+  destruct ρ as [ρ wfρ] ; cbn.
+  induction wfρ in n, Hdecl |- *.
+  - exists decl.
+    split.
+    1: easy.
+    reflexivity.
+  - cbn.
+    edestruct IHwfρ as [decl' [? IH]].
+    1: eassumption.
+    eexists ; split.
+    1: eassumption.
+    now rewrite <- rename_compose, <- compose_map_decl, IH, compose_map_decl, rename_compose.
+  - destruct n as [ | n].
+    + cbn in *.
+      inversion Hdecl ; subst ; clear Hdecl.
+      eexists ; split.
+      1: reflexivity.
+      unfold map_decl ; cbn.
+      f_equal.
+      rewrite <- rename_inst, rename_compose.
+      apply rename_ext.
+      intros ?.
+      now rewrite Nat.sub_0_r.
+    + cbn in *.
+      edestruct IHwfρ as [decl' [? IH]].
+      1: eassumption.
+      eexists ; split.
+      1: now rewrite Nat.sub_0_r.
+      now rewrite <- rename_compose, <- compose_map_decl, IH, compose_map_decl, rename_compose, Nat.sub_0_r.
+  Qed.
+
+Let PCon (Γ : context) := True.
+Let PTy (Γ : context) (A : term) := forall Δ (ρ : Δ ≤ Γ), [|- Δ ] -> [Δ |- A.[ren ρ]].
+Let PTm (Γ : context) (t A : term) := forall Δ (ρ : Δ ≤ Γ), [|- Δ ] ->
+  [Δ |- t.[ren ρ] : A.[ren ρ]].
+Let PTyEq (Γ : context) (A B : term) := forall Δ (ρ : Δ ≤ Γ), [|- Δ ] ->
+  [Δ |- A.[ren ρ] ≅ B.[ren ρ]].
+Let PTmEq (Γ : context) (t u A : term) := forall Δ (ρ : Δ ≤ Γ), [|- Δ ] ->
+  [Δ |- t.[ren ρ] ≅ u.[ren ρ] : A.[ren ρ]].
+
+
+Theorem typing_wk : wfInductionType PCon PTy PTm PTyEq PTmEq.
+Proof.
+  apply wfInduction.
+  - red.
+    trivial.
+  - red. trivial.
+  - intros ? ? IH.
+    now econstructor.
+  - intros Γ na A B HA IHA HB IHB Δ ρ HΔ.
+    econstructor ; fold inst.
+    1: easy.
+    replace (B.[up 1 (ren ρ)]) with (B.[ren (wk_lift ρ)])
+      by now rewrite ren_shiftn.
+    unshelve eapply (IHB _ {| wk := wk_lift ρ ; well_wk := _ |} _).
+    all: now econstructor.
+  - intros * _ IHA ? * ?.
+    econstructor.
+    now eapply IHA.
+  - intros * _ IHΓ Hnth ? * ?.
+    unshelve eapply nth_error_wk in Hnth as [decl' [? edecl]] ; tea.
+    unfold ren at 1.
+    cbn.
+    eapply termMetaConv.
+    1: econstructor ; eassumption.
+    rewrite <- rename_inst, ! lift_rename, rename_compose, (map_decl_type _ decl'), (map_decl_type _ decl).
+    f_equal.
+    rewrite ! lift_renaming_0_rshift, <- edecl.
+    eapply map_decl_ext ; intros ; eapply rename_ext ; intros ?.
+    now rewrite lift_renaming_0_rshift.
+  - intros * _ IHA _ IHB ? ρ ?.
+    cbn.
+    econstructor.
+    1: now eapply IHA.
+    replace B.[_] with B.[ren (wk_lift ρ)] by now rewrite ren_shiftn.
+    unshelve eapply (IHB _ {| wk := wk_lift ρ ; well_wk := _ |} _).
+    1: now econstructor.
+    econstructor ; tea.
+    econstructor.
+    now eapply IHA.
+  - intros * _ IHA _ IHt ? ρ ?.
+    cbn.
+    econstructor.
+    1: now eapply IHA.
+    red in IHt.
+    replace t.[_] with t.[ren (wk_lift ρ)] by now rewrite ren_shiftn.
+    replace B.[_] with B.[ren (wk_lift ρ)] by now rewrite ren_shiftn.
+    unshelve eapply (IHt _ {| wk := wk_lift ρ ; well_wk := _ |} _).
+    1: now econstructor.
+    econstructor ; tea.
+    now eapply IHA.
+  - intros * _ IHf _ IHu ? ρ ?.
+    cbn.
+    rewrite subst10_inst.
+    replace B.[_] with B.[(up 1 (ren ρ))] by (now rewrite up_Up).
+    econstructor.
+    2: now eapply IHu.
+    now eapply IHf.
+  - intros * _ IHt _ IHAB ? ρ ?.
+    econstructor.
+    1: now eapply IHt.
+    now eapply IHAB.
+  - intros Γ ? ? A A' B B' _ IHA _ IHAA' _ IHBB' ? ρ ?.
+    cbn.
+    econstructor.
+    + now eapply IHA.
+    + now eapply IHAA'.
+    + replace B.[_] with B.[ren (wk_lift ρ)] by now rewrite ren_shiftn.
+      replace B'.[_] with B'.[ren (wk_lift ρ)] by now rewrite ren_shiftn.
+      unshelve eapply (IHBB' _ {| wk := wk_lift ρ ; well_wk := _ |} _).
+      1: now econstructor.
+      econstructor ; tea.
+      now eapply IHA.
+  - intros * _ IHA ? ρ ?.
+    eapply TypeRefl.
+    now eapply IHA.
+  - intros * _ IH ? ρ ?.
+    econstructor.
+    now eapply IH.
+  - intros * _ IHA _ IHB ? ρ ?.
+    eapply TypeTrans.
+    + now eapply IHA.
+    + now eapply IHB.
+  - intros * _ IH ? ρ ?.
+    eapply convUniv.
+    now eapply IH.
+  - intros Γ ? ? A A' B B' _ IHA _ IHAA' _ IHBB' ? ρ ?.
+    cbn.
+    econstructor.
+    + now eapply IHA.
+    + now eapply IHAA'.
+    + replace B.[_] with B.[ren (wk_lift ρ)] by now rewrite ren_shiftn.
+      replace B'.[_] with B'.[ren (wk_lift ρ)] by now rewrite ren_shiftn.
+      unshelve eapply (IHBB' _ {| wk := wk_lift ρ ; well_wk := _ |} _).
+      all: now econstructor.
+  - intros Γ ? u u' f f' A B _ IHf _ IHu ? ρ ?.
+    cbn.
+    rewrite subst10_inst.
+    replace B.[_] with B.[(up 1 (ren ρ))] by (now rewrite up_Up).
+    now econstructor.
+  - intros Γ ? u t A B _ IHA _ IHt _ IHu ? ρ ?.
+    cbn. 
+    rewrite ! subst10_inst.
+    replace t.[⇑ _] with t.[(up 1 (ren ρ))] by (now rewrite up_Up).
+    replace t.[_] with t.[ren (wk_lift ρ)] by (now rewrite ren_shiftn).
+    replace B.[_] with B.[ren (wk_lift ρ)] by (now rewrite <- up_Up, ren_shiftn).
+    econstructor.
+    1,3: easy.
+    unshelve eapply (IHt _ {| wk := wk_lift ρ ; well_wk := _ |} _).
+    all: now econstructor.
+  - intros Γ ? ? f f' A B _ IHA _ IHf _ IHg _ IHe ? ρ ?.
+    cbn.
+    econstructor.
+    1-3: easy.
+    unshelve epose proof (IHe _ {| wk := wk_lift ρ ; well_wk := _ |} _) as IHe'.
+    2: now econstructor.
+    1: now econstructor.
+    cbn in *.
+    unfold ren in IHe' at 3 5.
+    unfold eta_expand.
+    cbn in *.
+    rewrite ! lift0_inst, ! inst_assoc in IHe' |- *.
+    replace B.[_] with B.[ren (shiftn 1 ρ)] by (now rewrite ren_shiftn).
+    unshelve erewrite (inst_ext _ _ _ f), (inst_ext _ _ _ f').
+    5: eassumption.
+    all: rewrite <- Upn_ren.
+    all: change 1 with (0 + 1).
+    all: rewrite <- subst_shift_comm.
+    all: cbn.
+    all: now rewrite Upn_0.
+  - intros * _ IHt ? ρ ?.
+    now econstructor.
+  - intros * _ IHt ? ρ ?.
+    now econstructor.
+  - intros * _ IHt _ IHt' ? ρ ?.
+    now eapply TermTrans.
+  - intros * _ IHt _ IHA ? ρ ?.
+    now eapply TermConv.
+Qed.
+
+End TypingWk.
